src/GoExamples.v
@@ -181,10 +181,12 @@ Local Open Scope map_scope.
 
 Definition swap_env : Env :=
   ("swap" -s> {|
-           ParamVars := [(Go.Num, 0); (Go.Num, 1)];
-           RetParamVars := []; Body := projT1 (extract_swap_prog (StringMap.empty _));
-           (* ret_not_in_args := ltac:(auto); *) args_no_dup := ltac:(auto); body_source := ltac:(repeat constructor);
-         |}; (StringMap.empty _)).
+     NumParamVars := 2;
+     NumRetParamVars := 0;
+     ParamVars := ((PassedByValue, Go.Num), (PassedByValue, Go.Num));
+     RetParamVars := tt; Body := projT1 (extract_swap_prog (StringMap.empty _));
+     (* ret_not_in_args := ltac:(auto); *) body_source := ltac:(repeat constructor);
+   |}; (StringMap.empty _)).
 
 Lemma swap_func : voidfunc2 "swap" swap_prog swap_env.
 Proof.
@@ -340,23 +342,6 @@ Example swap_example : stmt :=
   }
 *)
 
-Example swap_function_body : stmt :=
-  (Declare DiskBlock (fun va =>
-    (DiskRead va (Var 0);
-     Declare DiskBlock (fun vb =>
-      (DiskRead vb (Var 1);
-       DiskWrite (Var 0) (Var vb);
-       DiskWrite (Var 1) (Var va)))
-   )))%go.
-
-Example swap_function : OperationalSpec :=
-  {|
-    ParamVars := [(Go.Num, 0); (Go.Num, 1)];
-    RetParamVars := [];
-    Body := swap_function_body;
-    args_no_dup := ltac:(auto); body_source := ltac:(repeat constructor);
-  |}.
-
 Definition empty_env : Env := StringMap.empty _.
 
 (* Corresponding Go:
@@ -379,19 +364,21 @@ Example rot3_function_body : stmt :=
     (var0 <~const 1;
      Declare Num (fun var1 =>
       (var1 <~const 0;
-       Call [] "swap" [var1; var0]))));
+       Call 2 0 tt "swap" (var1, var0)))));
    Declare Num (fun var0 =>
     (var0 <~const 2;
      Declare Num (fun var1 =>
       (var1 <~const 1;
-       Call [] "swap" [var1; var0])))))%go.
+       Call 2 0 tt "swap" (var1, var0))))))%go.
 
-Example rot3_function : OperationalSpec :=
+Example rot3_function : FunctionSpec :=
   {|
-    ParamVars := [];
-    RetParamVars := [];
+    NumParamVars := 0;
+    NumRetParamVars := 0;
+    ParamVars := tt;
+    RetParamVars := tt;
     Body := rot3_function_body;
-    args_no_dup := ltac:(auto); body_source := ltac:(repeat constructor);
+    body_source := ltac:(repeat constructor);
   |}.
 
 (* Corresponding Go:
